LC_Barendregt_Enhanced_Instance.thy
@@ -1,0 +1,431 @@
+theory LC_Barendregt_Enhanced_Instance
+  imports "thys/MRBNF_Recursor" "HOL-Library.FSet"
+begin 
+
+(* binder_datatype 'a term =
+  Var 'a
+| App "'a term" "'a term"
+| Abs x::'a t::"'a term" binds x in t
+*)
+
+ML \<open>
+val ctors = [
+  (("Var", (NONE : mixfix option)), [@{typ 'var}]),
+  (("App", NONE), [@{typ 'rec}, @{typ 'rec}]),
+  (("Abs", NONE), [@{typ 'bvar}, @{typ 'brec}])
+]
+
+val spec = {
+  fp_b = @{binding "term"},
+  vars = [
+    (dest_TFree @{typ 'var}, MRBNF_Def.Free_Var),
+    (dest_TFree @{typ 'bvar}, MRBNF_Def.Bound_Var),
+    (dest_TFree @{typ 'brec}, MRBNF_Def.Live_Var),
+    (dest_TFree @{typ 'rec}, MRBNF_Def.Live_Var)
+  ],
+  binding_rel = [[0]],
+  rec_vars = 2,
+  ctors = ctors,
+  map_b = @{binding vvsubst},
+  tvsubst_b = @{binding tvsubst}
+}
+\<close>
+
+declare [[mrbnf_internals]]
+local_setup \<open>fn lthy =>
+let
+  val lthy' = MRBNF_Sugar.create_binder_datatype spec lthy
+in lthy' end\<close>
+print_mrbnfs
+
+(* unary substitution *)
+lemma IImsupp_VVr_empty: "IImsupp VVr = {}"
+  unfolding IImsupp_def SSupp_VVr_empty UN_empty Un_empty_left
+  apply (rule refl)
+  done
+
+lemma tvsubst_VVr_func: "tvsubst VVr t = t"
+  apply (rule term.TT_plain_co_induct)
+  subgoal for x
+    apply (rule case_split[of "isVVr (term_ctor x)"])
+     apply (unfold isVVr_def)[1]
+     apply (erule exE)
+    subgoal premises prems for a
+      unfolding prems
+      apply (rule tvsubst_VVr)
+      apply (rule SSupp_VVr_bound)
+        done
+      apply (rule trans)
+       apply (rule tvsubst_cctor_not_isVVr)
+          apply (rule SSupp_VVr_bound)
+      unfolding IImsupp_VVr_empty
+         apply (rule Int_empty_right)
+      unfolding tvnoclash_term_def Int_Un_distrib Un_empty
+        apply (rule conjI)
+         apply (rule iffD2[OF disjoint_iff], rule allI, rule impI, assumption)
+        apply (rule iffD2[OF disjoint_iff], rule allI, rule impI)
+      unfolding UN_iff Set.bex_simps
+        apply (rule ballI)
+        apply assumption+
+      apply (rule arg_cong[of _ _ term_ctor])
+      apply (rule trans)
+      apply (rule term_pre.map_cong)
+                 apply (rule supp_id_bound bij_id)+
+           apply (assumption | rule refl)+
+      unfolding id_def[symmetric] term_pre.map_id
+      apply (rule refl)
+      done
+    done
+
+lemma finite_singleton: "finite {x}" by blast
+lemma singl_bound: "|{a}| <o |UNIV::'a::var_term_pre set|"
+  by (rule finite_ordLess_infinite2[OF finite_singleton cinfinite_imp_infinite[OF term_pre.UNIV_cinfinite]])
+
+lemma SSupp_upd_bound:
+  fixes f::"'a::var_term_pre \<Rightarrow> 'a term"
+  shows "|SSupp (f (a:=t))| <o |UNIV::'a set| \<longleftrightarrow> |SSupp f| <o |UNIV::'a set|"
+  unfolding SSupp_def
+  apply (auto simp only: fun_upd_apply singl_bound ordLeq_refl split: if_splits
+      elim!: ordLeq_ordLess_trans[OF card_of_mono1 ordLess_ordLeq_trans[OF term_pre.Un_bound], rotated]
+      intro: card_of_mono1)
+  done
+
+corollary SSupp_upd_VVr_bound: "|SSupp (VVr(a:=(t::'a::var_term_pre term)))| <o |UNIV::'a set|"
+  apply (rule iffD2[OF SSupp_upd_bound])
+  apply (rule SSupp_VVr_bound)
+  done
+
+lemma fvars_subset_id_on: "supp f \<subseteq> A \<Longrightarrow> id_on (B - A) f"
+  unfolding supp_def id_on_def by blast
+
+lemma rrename_simps:
+  assumes "bij (f::'a::var_term_pre \<Rightarrow> 'a)" "|supp f| <o |UNIV::'a set|"
+  shows "rrename_term f (Var a) = Var (f a)"
+    "rrename_term f (App e1 e2) = App (rrename_term f e1) (rrename_term f e2)"
+    "rrename_term f (Abs x e) = Abs (f x) (rrename_term f e)"
+  unfolding Var_def App_def Abs_def term.rrename_cctors[OF assms] map_term_pre_def comp_def
+    Abs_term_pre_inverse[OF UNIV_I] map_sum_def sum.case map_prod_def prod.case id_def
+    apply (rule refl)+
+  done
+
+lemma App_inject[simp]: "(App a b = App c d) = (a = c \<and> b = d)"
+proof
+  assume "App a b = App c d"
+  then show "a = c \<and> b = d"
+    unfolding App_def fun_eq_iff term.TT_injects0
+      map_term_pre_def comp_def Abs_term_pre_inverse[OF UNIV_I] map_sum_def sum.case prod.map_id
+      Abs_term_pre_inject[OF UNIV_I UNIV_I]
+    by blast
+qed simp
+lemma Var_inject[simp]: "(Var a = Var b) = (a = b)"
+  apply (rule iffI[rotated])
+   apply (rule arg_cong[of _ _ Var])
+  apply assumption
+  unfolding Var_def term.TT_injects0 map_term_pre_def comp_def map_sum_def sum.case Abs_term_pre_inverse[OF UNIV_I]
+  id_def Abs_term_pre_inject[OF UNIV_I UNIV_I] sum.inject
+  apply (erule exE conjE)+
+  apply assumption
+  done
+lemma Abs_inject: "(Abs x e = Abs x' e') = (\<exists>f. bij f \<and> |supp (f::'a::var_term_pre \<Rightarrow> 'a)| <o |UNIV::'a set|
+  \<and> id_on (FFVars_term (Abs x e)) f \<and> f x = x' \<and> rrename_term f e = e')"
+  unfolding term.set
+  unfolding Abs_def term.TT_injects0 map_term_pre_def comp_def Abs_term_pre_inverse[OF UNIV_I]
+    map_sum_def sum.case map_prod_def prod.case id_def Abs_term_pre_inject[OF UNIV_I UNIV_I] sum.inject prod.inject
+    set3_term_pre_def sum_set_simps Union_empty Un_empty_left prod_set_simps cSup_singleton set2_term_pre_def
+    Un_empty_right UN_single
+  apply (rule refl)
+  done
+
+lemma bij_map_term_pre: "bij f \<Longrightarrow> |supp (f::'a::var_term_pre \<Rightarrow> 'a)| <o |UNIV::'a set| \<Longrightarrow> bij (map_term_pre (id::_::var_term_pre \<Rightarrow> _) f (rrename_term f) id)"
+  apply (rule iffD2[OF bij_iff])
+    apply (rule exI[of _ "map_term_pre id (inv f) (rrename_term (inv f)) id"])
+  apply (frule bij_imp_bij_inv)
+  apply (frule supp_inv_bound)
+   apply assumption
+  apply (rule conjI)
+   apply (rule trans)
+    apply (rule term_pre.map_comp0[symmetric])
+         apply (assumption | rule supp_id_bound)+
+  unfolding id_o inv_o_simp1 term.rrename_comp0s term.rrename_id0s
+  apply (rule term_pre.map_id0)
+  apply (rule trans)
+   apply (rule term_pre.map_comp0[symmetric])
+        apply (assumption | rule supp_id_bound)+
+  unfolding id_o inv_o_simp2 term.rrename_comp0s term.rrename_id0s
+  apply (rule term_pre.map_id0)
+  done
+
+lemma map_term_pre_inv_simp: "bij f \<Longrightarrow> |supp (f::'a::var_term_pre \<Rightarrow> 'a)| <o |UNIV::'a set| \<Longrightarrow> inv (map_term_pre (id::_::var_term_pre \<Rightarrow> _) f (rrename_term f) id) = map_term_pre id (inv f) (rrename_term (inv f)) id"
+  apply (frule bij_imp_bij_inv)
+  apply (frule supp_inv_bound)
+  apply assumption
+  apply (rule inv_unique_comp)
+   apply (rule trans)
+    apply (rule term_pre.map_comp0[symmetric])
+         apply (assumption | rule supp_id_bound)+
+   defer
+  apply (rule trans)
+    apply (rule term_pre.map_comp0[symmetric])
+         apply (assumption | rule supp_id_bound)+
+  unfolding id_o inv_o_simp1 inv_o_simp2 term.rrename_comp0s term.rrename_id0s term_pre.map_id0
+   apply (rule refl)+
+  done
+
+lemma Abs_set3: "term_ctor v = Abs x e \<Longrightarrow> \<exists>x' e'. term_ctor v = Abs x' e' \<and> x' \<in> set2_term_pre v \<and> e' \<in> set3_term_pre v"
+  unfolding Abs_def term.TT_injects0
+  apply (erule exE)
+  apply (erule conjE)+
+  subgoal for f
+apply (drule iffD2[OF bij_imp_inv', rotated, of "map_term_pre id f (rrename_term f) id"])
+     apply (rule bij_map_term_pre)
+      apply assumption+
+    apply (rule exI)
+    apply (rule exI)
+    apply (rule conjI)
+     apply (rule exI[of _ "id"])
+     apply (rule conjI bij_id supp_id_bound id_on_id)+
+    apply (drule sym)
+    unfolding term.rrename_id0s term_pre.map_id map_term_pre_inv_simp
+    unfolding map_term_pre_def comp_def Abs_term_pre_inverse[OF UNIV_I] map_sum_def sum.case
+      map_prod_def prod.case id_def
+    apply assumption
+    apply (raw_tactic \<open>hyp_subst_tac @{context} 1\<close>)
+unfolding set2_term_pre_def set3_term_pre_def comp_def Abs_term_pre_inverse[OF UNIV_I] sum_set_simps
+    map_sum_def sum.case Union_empty Un_empty_left map_prod_def prod.case prod_set_simps
+      ccpo_Sup_singleton Un_empty_right id_on_def image_single[symmetric]
+  unfolding term.FFVars_rrenames[OF bij_imp_bij_inv supp_inv_bound]
+  unfolding image_single image_set_diff[OF bij_is_inj[OF bij_imp_bij_inv], symmetric]
+    image_in_bij_eq[OF bij_imp_bij_inv] inv_inv_eq image_in_bij_eq[OF term.rrename_bijs[OF bij_imp_bij_inv supp_inv_bound]]
+  term.rrename_inv_simps[OF bij_imp_bij_inv supp_inv_bound] inv_simp2
+  unfolding term.rrename_comps[OF bij_imp_bij_inv supp_inv_bound] inv_o_simp2 term.rrename_ids
+  apply (rule conjI bij_imp_bij_inv supp_inv_bound singletonI | assumption)+
+  done
+  done
+
+lemma Abs_avoid: "|A::'a::var_term_pre set| <o |UNIV::'a set| \<Longrightarrow> \<exists>x' e'. Abs x e = Abs x' e' \<and> x' \<notin> A"
+  apply (drule term.TT_fresh_nchotomys[of _ "Abs x e"])
+  apply (erule exE)
+  apply (erule conjE)
+   apply (drule sym)
+  apply (frule Abs_set3)
+  apply (erule exE conjE)+
+  apply (rule exI)+
+  apply (rule conjI)
+   apply (rule trans)
+    apply (rule sym)
+    apply assumption
+  apply (rotate_tac 2)
+   apply assumption
+  apply (drule iffD1[OF disjoint_iff])
+  apply (erule allE)
+  apply (erule impE)
+   apply assumption
+  apply assumption
+  done
+
+lemma VVr_eq_Var: "VVr a = Var a"
+  unfolding VVr_def Var_def comp_def \<eta>_def
+  by (rule refl)
+
+lemma rrename_term_simps[simp]: 
+"bij (\<sigma>::'a\<Rightarrow>'a) \<Longrightarrow> |supp \<sigma>| <o |UNIV:: 'a::var_term_pre set| \<Longrightarrow> 
+ rrename_term \<sigma> (Var a) = Var (\<sigma> a)"
+"bij (\<sigma>::'a\<Rightarrow>'a) \<Longrightarrow> |supp \<sigma>| <o |UNIV:: 'a::var_term_pre set| \<Longrightarrow> 
+ rrename_term \<sigma> (App e1 e2) = App (rrename_term \<sigma> e1) (rrename_term \<sigma> e2)"
+"bij (\<sigma>::'a\<Rightarrow>'a) \<Longrightarrow> |supp \<sigma>| <o |UNIV:: 'a::var_term_pre set| \<Longrightarrow> 
+ rrename_term \<sigma> (Abs a e) = Abs (\<sigma> a) (rrename_term \<sigma> e)"
+sorry
+
+find_theorems tvsubst 
+lemma rrename_term_tvsubst: "bij (\<sigma>::'a\<Rightarrow>'a) \<Longrightarrow> |supp \<sigma>| <o |UNIV:: 'a::var_term_pre set| \<Longrightarrow>  
+     |SSupp \<tau>| <o |UNIV:: 'a::var_term_pre set| \<Longrightarrow>
+     rrename_term \<sigma> (tvsubst \<tau> e) = tvsubst (rrename_term \<sigma> \<circ> \<tau>) (rrename_term \<sigma> e)"
+sorry
+
+lemma tvsubst_o: "|SSupp \<sigma>| <o |UNIV:: 'a::var_term_pre set| \<Longrightarrow>  
+     |SSupp \<tau>| <o |UNIV:: 'a::var_term_pre set| \<Longrightarrow>
+     tvsubst \<sigma> (tvsubst \<tau> e) = tvsubst (tvsubst \<sigma> \<circ> \<tau>) e"
+sorry
+
+lemma [simp]: "bij (\<sigma>::'a\<Rightarrow>'a) \<Longrightarrow> |supp \<sigma>| <o |UNIV:: 'a::var_term_pre set| \<Longrightarrow>  
+      rrename_term \<sigma> o (VVr(a := e)) = VVr (\<sigma> a := rrename_term \<sigma> e)"
+sorry
+
+lemmas SSupp_upd_VVr_bound[simp,intro]
+lemmas supp_inv_bound[simp]
+lemmas term.rrename_ids[simp]
+lemmas bij_swap[simp]
+
+lemma supp_swap_bound[intro]: "|supp (id(x::'a := xx, xx := x))| <o |UNIV:: 'a::var_term_pre set|"
+by (simp add: cinfinite_imp_infinite supp_swap_bound term.UNIV_cinfinite)
+
+lemmas supp_id_bound[simp]
+
+lemma rrename_term_cong_id[simp]: 
+"bij (\<sigma>::'a\<Rightarrow>'a) \<Longrightarrow> |supp \<sigma>| <o |UNIV:: 'a::var_term_pre set| \<Longrightarrow>   
+ \<forall>a\<in>FFVars_term e. \<sigma> a = (a::'a) \<Longrightarrow> rrename_term \<sigma> e = e"
+sorry
+
+lemma Abs_rrename_term: 
+"bij (\<sigma>::'a\<Rightarrow>'a) \<Longrightarrow> |supp \<sigma>| <o |UNIV:: 'a::var_term_pre set| \<Longrightarrow>   
+ \<forall>a'\<in>FFVars_term e - {a::'a}. \<sigma> a' = a' \<Longrightarrow> Abs a e = Abs (\<sigma> a) (rrename_term \<sigma> e)"
+sorry
+
+lemma tvsubst_VVr_rrename_term: 
+"xx \<notin> FFVars_term e1 - {x} \<Longrightarrow> 
+ tvsubst (VVr((x::'a::var_term_pre) := e2)) e1 = tvsubst (VVr(xx := e2)) (rrename_term (id(x := xx, xx := x)) e1)"
+sorry
+ 
+
+(* AN EXAMPLE INDUCTIVE DEFINITION *)
+(* (a reduced form of) small step semantics *) 
+
+inductive step :: "'a::var_term_pre term \<times> 'a term \<Rightarrow> bool" where
+  Beta: "step (App (Abs x e) e2, tvsubst (VVr(x:=e2)) e)"
+| AppL: "step (e1,e1') \<Longrightarrow> step (App e1 e2, App e1' e2)"
+| Xi: "step (e,e') \<Longrightarrow> step (Abs x e, Abs x e')"
+
+lemmas step_def = nitpick_unfold(173)
+
+
+(* INSTANTIATING THE ABSTRACT SETTING: *)
+
+type_synonym 'a T = "'a term \<times> 'a term"
+type_synonym 'a V = "'a list"
+
+definition "small (A::'a set) \<equiv> |A| <o |UNIV::'a set|" 
+definition "ssbij f \<equiv> bij f \<and> small (supp (f::'a::var_term_pre \<Rightarrow> 'a))" 
+
+definition Tmap :: "('a::var_term_pre \<Rightarrow> 'a) \<Rightarrow> 'a T \<Rightarrow> 'a T" where 
+"Tmap f \<equiv> map_prod (rrename_term f) (rrename_term f)"
+
+fun Tfvars :: "('a::var_term_pre) T \<Rightarrow> 'a set" where 
+"Tfvars (e1,e2) = FFVars_term e1 \<union> FFVars_term e2"
+
+definition Vmap :: "('a::var_term_pre \<Rightarrow> 'a) \<Rightarrow> 'a V \<Rightarrow> 'a V" where 
+"Vmap \<equiv> map"
+
+fun Vfvars :: "('a::var_term_pre) V \<Rightarrow> 'a set" where 
+"Vfvars v = set v"
+
+definition G :: "('a::var_term_pre T \<Rightarrow> bool) \<Rightarrow> 'a V \<Rightarrow> 'a T \<Rightarrow> bool"
+where
+"G \<equiv> \<lambda>R v t.  
+         (\<exists>x e1 e2. v = [x] \<and> fst t = App (Abs x e1) e2 \<and> snd t = tvsubst (VVr(x := e2)) e1)
+         \<or>
+         (\<exists>e1 e1' e2. v = [] \<and> fst t = App e1 e2 \<and> snd t = App e1' e2 \<and> R (e1,e1')) 
+         \<or>
+         (\<exists>x e e'. v = [x] \<and> fst t = Abs x e \<and> snd t = Abs x e' \<and> R (e,e'))"
+
+lemma step_G: "step = lfp (\<lambda>R t. \<exists>v. G R v t)" 
+  unfolding step_def G_def apply(rule arg_cong[of _ _  lfp])
+  unfolding fun_eq_iff by simp (smt (verit))
+
+
+(* VERIFYING THE HYPOTHESES FOR BARENDREGT-ENHANCED INDUCTION: *)
+
+lemma G_mono: "\<And>R R' k v t. R \<le> R' \<Longrightarrow> G R v t \<Longrightarrow> G R' v t"
+unfolding G_def by fastforce
+
+lemma G_equiv: "\<And>\<sigma> R v t. ssbij \<sigma> \<Longrightarrow> G R v t \<Longrightarrow> G (\<lambda>t'. R (Tmap (inv \<sigma>) t')) (Vmap \<sigma> v) (Tmap \<sigma> t)"
+unfolding G_def subgoal for \<sigma> R v t apply(elim disjE)
+  subgoal apply(rule disjI1)
+  subgoal apply(elim exE) subgoal for x e1 e2 
+  apply(rule exI[of _ "\<sigma> x"])
+  apply(rule exI[of _ "rrename_term \<sigma> e1"]) apply(rule exI[of _ "rrename_term \<sigma> e2"])
+  apply(cases t) unfolding ssbij_def small_def Tmap_def Vmap_def apply simp
+  apply(subst rrename_term_tvsubst) by auto . .
+  (* *)
+  subgoal apply(rule disjI2, rule disjI1)
+  subgoal apply(elim exE) subgoal for e1 e1' e2
+  apply(rule exI[of _ "rrename_term \<sigma> e1"]) apply(rule exI[of _ "rrename_term \<sigma> e1'"]) 
+  apply(rule exI[of _ "rrename_term \<sigma> e2"])
+  apply(cases t) unfolding ssbij_def small_def Tmap_def Vmap_def 
+  by (simp add: term.rrename_comps) . . 
+  (* *)
+  subgoal apply(rule disjI2, rule disjI2)
+  subgoal apply(elim exE) subgoal for x e e'
+  apply(rule exI[of _ "\<sigma> x"])
+  apply(rule exI[of _ "rrename_term \<sigma> e"]) apply(rule exI[of _ "rrename_term \<sigma> e'"]) 
+  apply(cases t) unfolding ssbij_def small_def Tmap_def Vmap_def 
+  by (simp add: term.rrename_comps) . . . .
+
+lemma fresh: "\<exists>xx. xx \<notin> Tfvars t"  
+by (metis Abs_avoid Tfvars.elims term.card_of_FFVars_bounds term.set(2))
+
+lemma G_fresh: 
+"\<And>R v t. (\<forall>\<sigma> t. ssbij \<sigma> \<and> R t \<longrightarrow> R (Tmap \<sigma> t)) \<Longrightarrow> G R v t \<Longrightarrow> 
+         \<exists>w. Vfvars w  \<inter> Tfvars t = {} \<and> G R w t"
+subgoal for R v t
+using fresh[of t] unfolding G_def Tmap_def Vmap_def apply safe
+  subgoal for xx x e1 e2
+  apply(rule exI[of _ "[xx]"])  
+  apply(rule conjI)
+    subgoal unfolding ssbij_def small_def Vmap_def by auto 
+    subgoal apply(rule disjI1) 
+    apply(rule exI[of _ "xx"]) 
+    apply(rule exI[of _ "rrename_term (id(x:=xx,xx:=x)) e1"])
+    apply(rule exI[of _ "e2"])
+    apply(cases t)  apply simp apply(intro conjI)
+      subgoal apply(subst Abs_rrename_term[of "id(x:=xx,xx:=x)"]) by auto
+      subgoal apply(subst tvsubst_VVr_rrename_term) by auto . .
+  subgoal for xx e1 e1' e2
+  apply(rule exI[of _ "[]"])  
+  apply(rule conjI)
+    subgoal unfolding ssbij_def small_def Vmap_def by auto 
+    subgoal apply(rule disjI2, rule disjI1) 
+    apply(rule exI[of _ "e1"]) 
+    apply(rule exI[of _ "e1'"])
+    apply(rule exI[of _ "e2"]) 
+    apply(cases t)  apply simp . .
+  subgoal for xx x e e'
+  apply(rule exI[of _ "[xx]"])  
+  apply(rule conjI)
+    subgoal unfolding ssbij_def small_def Vmap_def by auto 
+    subgoal apply(rule disjI2, rule disjI2) 
+    apply(rule exI[of _ "xx"]) 
+    apply(rule exI[of _ "rrename_term (id(x:=xx,xx:=x)) e"])
+    apply(rule exI[of _ "rrename_term (id(x:=xx,xx:=x)) e'"])
+    apply(cases t)  apply simp apply(intro conjI)
+      subgoal apply(subst Abs_rrename_term[of "id(x:=xx,xx:=x)"]) by auto
+      subgoal apply(subst Abs_rrename_term[of "id(x:=xx,xx:=x)"]) by auto
+      subgoal by (metis supp_swap_bound Prelim.bij_swap small_def ssbij_def) . . . .
+
+
+(* WHAT THE ABSTRACT SETTING GIVES US: *)
+typedecl 'a P (* parameters *)
+consts Pfvars :: "('a::var_term_pre) P \<Rightarrow> 'a set"
+
+axiomatization where  
+small_Pfvars: "\<And>p. small (Pfvars p)" 
+
+theorem BE_induct: 
+assumes I: "step (t::('a::var_term_pre) T)"
+and strong: "\<And> p v t. Vfvars v \<inter> Pfvars p = {} \<Longrightarrow> Vfvars v \<inter> Tfvars t = {} \<Longrightarrow> 
+      G (\<lambda>t'. step t' \<and> (\<forall>p'. R p' t')) v t \<Longrightarrow> R p t"
+shows "R p t"
+sorry
+
+(* FROM ABSTRACT BACK TO CONCRETE: *)
+thm step.induct[no_vars]
+
+(*
+corollary just_some_sanity_check: "step t \<Longrightarrow>
+(\<And>x e e2 p. R p (App (Abs x e) e2, tvsubst (VVr(x := e2)) e)) \<Longrightarrow>
+(\<And>e1 e1' e2 p. step (e1, e1') \<Longrightarrow> (\<forall>p'. R p' (e1, e1')) \<Longrightarrow> R p (App e1 e2, App e1' e2)) \<Longrightarrow> 
+(\<And>e e' x p. step (e, e') \<Longrightarrow> (\<forall>p'. R p' (e, e')) \<Longrightarrow> R p (Abs x e, Abs x e')) \<Longrightarrow> 
+ R p t"
+subgoal premises p using p(1) apply(induct arbitrary: p rule: step.induct) 
+using p(2-) by auto .
+*)
+
+corollary BE_induct_step: "step t \<Longrightarrow>
+(\<And>x e e2 p. x \<notin> Pfvars p \<Longrightarrow> x \<notin> FFVars_term e2 \<Longrightarrow> R p (App (Abs x e) e2, tvsubst (VVr(x := e2)) e)) \<Longrightarrow>
+(\<And>e1 e1' e2 p. step (e1, e1') \<Longrightarrow> (\<forall>p'. R p' (e1, e1')) \<Longrightarrow> R p (App e1 e2, App e1' e2)) \<Longrightarrow> 
+(\<And>e e' x p. x \<notin> Pfvars p \<Longrightarrow> step (e, e') \<Longrightarrow> (\<forall>p'. R p' (e, e')) \<Longrightarrow> R p (Abs x e, Abs x e')) \<Longrightarrow> 
+ R p t"
+apply(erule BE_induct)
+unfolding G_def by auto
+      
+
+end
